Return and bind for IO monad are now written in C

benchmarks/io/prog_main.c
@@ -9,25 +9,25 @@ extern void body(struct thread_info *);
 extern value args[];
 
 extern struct thread_info;
-extern void print_Coq_Init_Datatypes_bool(value);
-extern value get_Coq_Init_Datatypes_pair_args(value);
 extern value get_Coq_Strings_String_string_tag(value);
 extern value get_Coq_Init_Datatypes_bool_tag(value);
 extern value make_Coq_Init_Datatypes_bool_true(void);
 extern value make_Coq_Init_Datatypes_bool_false(void);
 extern value make_Coq_Init_Datatypes_unit_tt(void);
 extern value make_Coq_Strings_String_string_EmptyString(void);
-extern value make_Coq_Strings_String_string_String(value, value, value**);
 extern value alloc_make_Coq_Strings_Ascii_ascii_Ascii(struct thread_info *, value, value, value, value, value, value, value, value);
 extern value alloc_make_Coq_Strings_String_string_String(struct thread_info *, value, value);
-extern void print_Coq_Init_Datatypes_unit(value);
-extern void* call(struct thread_info *tinfo, value clos, value arg0);
-extern value make_Top_FFI_Build_FFI(value, value, value, value**);
 
+extern value alloc_make_Top_IO_Types_Build_IO_Types(struct thread_info *, value, value);
+extern value alloc_make_Top_IO_Impl_Build_IO_Impl(struct thread_info *, value, value);
+extern value alloc_make_Top_StringFFI_Build_StringFFI(struct thread_info *, value, value);
+
+extern void* call(struct thread_info *tinfo, value clos, value arg0);
+
+extern value const io_ret_clo[2];
+extern value const io_bind_clo[2];
 extern value const print_string_clo[2];
 extern value const scan_string_clo[2];
-extern value const print_time_clo[2];
-
 
 _Bool is_ptr(value s) {
   return (_Bool) Is_block(s);
@@ -94,13 +94,6 @@ value scan_string(struct thread_info *tinfo) {
   return s;
 }
 
-value print_time(struct thread_info *tinfo) { 
-  clock_t now = clock();
-  printf("%lu\n", now);
-  fflush(stdout);
-  return make_Coq_Init_Datatypes_unit_tt(); 
-}
-
 value calls(struct thread_info* tinfo, value clos, unsigned int n, ...)
 {
   value v = clos;
@@ -114,6 +107,19 @@ value calls(struct thread_info* tinfo, value clos, unsigned int n, ...)
   va_end(args);
   return clos;
 }
+
+value io_ret(struct thread_info * tinfo, value sigma, value x) {
+  return x;
+}
+
+value io_bind(struct thread_info * tinfo, value sigma, value tau, value x, value f) {
+  call(tinfo, x, 1);
+  // dereference to get the first thing in A * World
+  value out = *((value *) tinfo->args[1]);
+  calls(tinfo, f, 2, out, 1);
+  return *((value *) tinfo->args[1]);
+}
+
 
 /* Main */
 int main(int argc, char *argv[]) {
@@ -129,19 +135,23 @@ int main(int argc, char *argv[]) {
   body(tinfo);
   end = clock();
 
-  /* Get the andb function from the arguments array */
   clo = tinfo -> args[1];
 
-  value ffi[10];
-  value built_ffi = 
-    make_Top_FFI_Build_FFI(
+  // Types are dummy values
+  value io_types = alloc_make_Top_IO_Types_Build_IO_Types(tinfo, 1, 1);
+
+  value io_impl = alloc_make_Top_IO_Impl_Build_IO_Impl(tinfo, io_ret_clo, io_bind_clo);
+
+  value string_ffi = 
+    alloc_make_Top_StringFFI_Build_StringFFI(
+        tinfo,
         print_string_clo,
-        scan_string_clo,
-        print_time_clo,
-        ffi);
+        scan_string_clo);
+
+  // Worlds are dummy values in runtime
   value world = 1;
 
-  value v = calls(tinfo, clo, 2, built_ffi, world);
+  value v = calls(tinfo, clo, 4, io_types, io_impl, string_ffi, world);
 
   sec = (double)(end - start)/CLOCKS_PER_SEC;
   msec = 1000*sec;
