theories/Compiler/pipeline.v
@@ -97,14 +97,18 @@ Definition make_glue (opts : Options) (p : Template.Ast.program)
   : error (cps_util.name_env * Clight.program * Clight.program * list string)  :=
   match generate_glue opts p with
   | Ret (nenv, Some hdr, Some prg, logs) =>
-    Ret (nenv, hdr, prg, logs)
-  | _ => Err "Error in generating glue code"
+      Ret (nenv, hdr, prg, logs)
+  | Ret (nenv, _, _, logs) =>
+      Err "No Clight program generated"
+  | Err s => Err s
   end.
 
 Definition make_ffi (opts : Options) (p : Template.Ast.program)
   : error (cps_util.name_env * Clight.program * Clight.program * list string)  :=
   match generate_ffi opts p with
   | Ret (nenv, Some hdr, Some prg, logs) =>
-    Ret (nenv, hdr, prg, logs)
-  | _ => Err "Error in generating glue code"
+      Ret (nenv, hdr, prg, logs)
+  | Ret (nenv, _, _, logs) =>
+      Err "No Clight program generated"
+  | Err s => Err s
   end.
